Implement Hacl.Hash.SHA2.update_last through a generic, alg-paramteric combinator

code/hash/Hacl.Hash.SHA2.fst
@@ -226,260 +226,108 @@ let pad_256 = Hacl.Hash.PadFinish.pad SHA2_256
 let pad_384 = Hacl.Hash.PadFinish.pad SHA2_384
 let pad_512 = Hacl.Hash.PadFinish.pad SHA2_512
 
+inline_for_extraction noextract
+val mk_update_last: a:sha2_alg -> update_last_st (| a, () |)
+
 #push-options "--z3rlimit 300"
 
-let update_last_224 st prev_len input input_len =
+let mk_update_last a st prev_len input input_len =
   let h0 = ST.get () in
   [@inline_let]
-  let st' = coerce_to_mb_state SHA2_224 st in
+  let st' = coerce_to_mb_state a st in
   [@inline_let]
   let input' = ntup1 #(Lib.Buffer.lbuffer Lib.IntTypes.uint8 input_len) #1 input in
-  Lib.IntVector.reveal_vec_1 (word_t SHA2_224);
+  Lib.IntVector.reveal_vec_1 (word_t a);
   [@inline_let]
-  let totlen = prev_len `Hacl.Hash.MD.len_add32 SHA2_224` input_len in
-  Hacl.SHA2.Scalar32.sha224_update_last totlen input_len input' st';
+  let totlen = prev_len `Hacl.Hash.MD.len_add32 a` input_len in
+  begin match a with
+  | SHA2_224 -> Hacl.SHA2.Scalar32.sha224_update_last totlen input_len input' st'
+  | SHA2_256 -> Hacl.SHA2.Scalar32.sha256_update_last totlen input_len input' st'
+  | SHA2_384 -> Hacl.SHA2.Scalar32.sha384_update_last totlen input_len input' st'
+  | SHA2_512 -> Hacl.SHA2.Scalar32.sha512_update_last totlen input_len input' st'
+  end;
   let h1 = ST.get () in
   begin (* ghost *)
     let input0_raw = B.as_seq h0 input in
     let input0 = as_seq_multi h0 input' in
 
     let st0 = as_seq h0 st in
-    let st0' = as_seq #(| SHA2_224, () |) h0 st' in
+    let st0' = as_seq #(| a, () |) h0 st' in
     let vlen = Lib.IntTypes.v input_len in
     let vprev_len = prev_len_v prev_len in
-    let vtotlen = Lib.IntTypes.v totlen in
-    let pad_s = Spec.Hash.MD.pad SHA2_224 vtotlen in
+    let vtotlen = len_v a totlen in
+    let pad_s = Spec.Hash.MD.pad a vtotlen in
     let blocks1 = Seq.append input0 pad_s in
     let blocks1_raw = Seq.append input0_raw pad_s in
-    assert (Seq.length blocks1 % block_length SHA2_224 == 0);
-    assert (Seq.length blocks1_raw % block_length SHA2_224 == 0);
+    calc (==) {
+      blocks1;
+      (==) { ntup1_lemma #_ #1 input0; assert (Seq.equal blocks1 blocks1_raw) }
+      blocks1_raw;
+    };
+
+    calc (==) {
+      vtotlen % block_length a;
+      (==) { }
+      (vprev_len + vlen) % block_length a;
+      (==) { Math.Lemmas.lemma_mod_add_distr vlen vprev_len (block_length a) }
+      vlen % block_length a;
+    };
+
+    calc (==) {
+      Seq.length blocks1 % block_length a;
+      (==) { }
+      (vlen + Seq.length pad_s) % block_length a;
+      (==) { Math.Lemmas.lemma_mod_add_distr (Seq.length pad_s) vlen (block_length a) }
+      (vlen % block_length a + Seq.length pad_s) % block_length a;
+      (==) { }
+      (vtotlen % block_length a + Seq.length pad_s) % block_length a;
+      (==) { Math.Lemmas.lemma_mod_add_distr (Seq.length pad_s) vtotlen (block_length a) }
+      (vtotlen + Seq.length pad_s) % block_length a;
+      (==) { }
+      0;
+    };
 
     calc (==) {
         as_seq h1 st;
       (==) { }
-        Vec.update_last #SHA2_224 #Vec.M32 totlen vlen input0 st0';
-      (==) { state_spec_v_lemma SHA2_224 (Vec.update_last totlen vlen input0 st0') }
-        Lib.Sequence.index (Vec.state_spec_v #SHA2_224 #Vec.M32 (Vec.update_last totlen vlen input0 st0')) 0;
-      (==) { Hacl.Spec.SHA2.Equiv.update_last_lemma_l #SHA2_224 #Vec.M32 totlen vlen input0 st0' 0 }
-        Hacl.Spec.SHA2.update_last SHA2_224 totlen vlen input0.(|0|)
-          (Lib.Sequence.index (Vec.state_spec_v #SHA2_224 #Vec.M32 st0') 0);
-      (==) { state_spec_v_lemma SHA2_224 st0' }
-        Hacl.Spec.SHA2.update_last SHA2_224 totlen vlen input0.(|0|) st0';
+        Vec.update_last #a #Vec.M32 totlen vlen input0 st0';
+      (==) { state_spec_v_lemma a (Vec.update_last totlen vlen input0 st0') }
+        Lib.Sequence.index (Vec.state_spec_v #a #Vec.M32 (Vec.update_last totlen vlen input0 st0')) 0;
+      (==) { Hacl.Spec.SHA2.Equiv.update_last_lemma_l #a #Vec.M32 totlen vlen input0 st0' 0 }
+        Hacl.Spec.SHA2.update_last a totlen vlen input0.(|0|)
+          (Lib.Sequence.index (Vec.state_spec_v #a #Vec.M32 st0') 0);
+      (==) { state_spec_v_lemma a st0' }
+        Hacl.Spec.SHA2.update_last a totlen vlen input0.(|0|) st0';
       (==) { ntup1_lemma #_ #1 input0 }
-        Hacl.Spec.SHA2.update_last SHA2_224 totlen vlen input0 st0';
+        Hacl.Spec.SHA2.update_last a totlen vlen input0 st0';
       (==) {
-        Hacl.Spec.SHA2.EquivScalar.update_last_is_repeat_blocks_multi SHA2_224 vtotlen vlen input0 st0'
+        Hacl.Spec.SHA2.EquivScalar.update_last_is_repeat_blocks_multi a vtotlen vlen input0 st0'
       }
-        Lib.Sequence.repeat_blocks_multi (block_length SHA2_224) blocks1 (Hacl.Spec.SHA2.update SHA2_224) st0';
+        Lib.Sequence.repeat_blocks_multi (block_length a) blocks1 (Hacl.Spec.SHA2.update a) st0';
       (==) { assert (st0 `Seq.equal` st0');
              ntup1_lemma #_ #1 input0; assert (blocks1 `Seq.equal` blocks1_raw) }
-        Lib.Sequence.repeat_blocks_multi (block_length SHA2_224) blocks1_raw (Hacl.Spec.SHA2.update SHA2_224) st0;
-      (==) { Classical.forall_intro_2 (Hacl.Spec.SHA2.EquivScalar.update_lemma SHA2_224);
-             Lib.Sequence.Lemmas.repeat_blocks_multi_extensionality (block_length SHA2_224)
+        Lib.Sequence.repeat_blocks_multi (block_length a) blocks1_raw (Hacl.Spec.SHA2.update a) st0;
+      (==) { Classical.forall_intro_2 (Hacl.Spec.SHA2.EquivScalar.update_lemma a);
+             Lib.Sequence.Lemmas.repeat_blocks_multi_extensionality (block_length a)
                blocks1_raw
-               (Hacl.Spec.SHA2.update SHA2_224)
-               (Lib.UpdateMulti.Lemmas.repeat_f (block_length SHA2_224) (Spec.Agile.Hash.update SHA2_224))
+               (Hacl.Spec.SHA2.update a)
+               (Lib.UpdateMulti.Lemmas.repeat_f (block_length a) (Spec.Agile.Hash.update a))
                st0 }
-        Lib.Sequence.repeat_blocks_multi (block_length SHA2_224) blocks1_raw
-          (Lib.UpdateMulti.Lemmas.repeat_f (block_length SHA2_224) (Spec.Agile.Hash.update SHA2_224))
+        Lib.Sequence.repeat_blocks_multi (block_length a) blocks1_raw
+          (Lib.UpdateMulti.Lemmas.repeat_f (block_length a) (Spec.Agile.Hash.update a))
           st0;
       (==) {
-        Lib.UpdateMulti.Lemmas.update_multi_is_repeat_blocks_multi (block_length SHA2_224) (Spec.Agile.Hash.update SHA2_224) st0 blocks1_raw }
-        Lib.UpdateMulti.mk_update_multi (block_length SHA2_224) (Spec.Agile.Hash.update SHA2_224) st0 blocks1_raw;
+        Lib.UpdateMulti.Lemmas.update_multi_is_repeat_blocks_multi (block_length a) (Spec.Agile.Hash.update a) st0 blocks1_raw }
+        Lib.UpdateMulti.mk_update_multi (block_length a) (Spec.Agile.Hash.update a) st0 blocks1_raw;
       (==) { }
-        Spec.Hash.Incremental.update_last SHA2_224 st0 (prev_len_v prev_len) input0_raw;
+        Spec.Hash.Incremental.update_last a st0 (prev_len_v prev_len) input0_raw;
     }
   end
 
-let update_last_256 st prev_len input input_len =
-  let h0 = ST.get () in
-  [@inline_let]
-  let st' = coerce_to_mb_state SHA2_256 st in
-  [@inline_let]
-  let input' = ntup1 #(Lib.Buffer.lbuffer Lib.IntTypes.uint8 input_len) #1 input in
-  Lib.IntVector.reveal_vec_1 (word_t SHA2_256);
-  [@inline_let]
-  let totlen = prev_len `Hacl.Hash.MD.len_add32 SHA2_256` input_len in
-  Hacl.SHA2.Scalar32.sha256_update_last totlen input_len input' st';
-  let h1 = ST.get () in
-  begin (* ghost *)
-    let input0_raw = B.as_seq h0 input in
-    let input0 = as_seq_multi h0 input' in
-
-    let st0 = as_seq h0 st in
-    let st0' = as_seq #(| SHA2_256, () |) h0 st' in
-    let vlen = Lib.IntTypes.v input_len in
-    let vprev_len = prev_len_v prev_len in
-    let vtotlen = Lib.IntTypes.v totlen in
-    let pad_s = Spec.Hash.MD.pad SHA2_256 vtotlen in
-    let blocks1 = Seq.append input0 pad_s in
-    let blocks1_raw = Seq.append input0_raw pad_s in
-    assert (Seq.length blocks1 % block_length SHA2_256 == 0);
-    assert (Seq.length blocks1_raw % block_length SHA2_256 == 0);
-
-
-    calc (==) {
-        as_seq h1 st;
-      (==) { }
-        Vec.update_last #SHA2_256 #Vec.M32 totlen vlen input0 st0';
-      (==) { state_spec_v_lemma SHA2_256 (Vec.update_last totlen vlen input0 st0') }
-        Lib.Sequence.index (Vec.state_spec_v #SHA2_256 #Vec.M32 (Vec.update_last totlen vlen input0 st0')) 0;
-      (==) { Hacl.Spec.SHA2.Equiv.update_last_lemma_l #SHA2_256 #Vec.M32 totlen vlen input0 st0' 0 }
-        Hacl.Spec.SHA2.update_last SHA2_256 totlen vlen input0.(|0|)
-          (Lib.Sequence.index (Vec.state_spec_v #SHA2_256 #Vec.M32 st0') 0);
-      (==) { state_spec_v_lemma SHA2_256 st0' }
-        Hacl.Spec.SHA2.update_last SHA2_256 totlen vlen input0.(|0|) st0';
-      (==) { ntup1_lemma #_ #1 input0 }
-        Hacl.Spec.SHA2.update_last SHA2_256 totlen vlen input0 st0';
-      (==) {
-        Hacl.Spec.SHA2.EquivScalar.update_last_is_repeat_blocks_multi SHA2_256 vtotlen vlen input0 st0'
-      }
-        Lib.Sequence.repeat_blocks_multi (block_length SHA2_256) blocks1 (Hacl.Spec.SHA2.update SHA2_256) st0';
-      (==) { assert (st0 `Seq.equal` st0');
-             ntup1_lemma #_ #1 input0; assert (blocks1 `Seq.equal` blocks1_raw) }
-        Lib.Sequence.repeat_blocks_multi (block_length SHA2_256) blocks1_raw (Hacl.Spec.SHA2.update SHA2_256) st0;
-      (==) { Classical.forall_intro_2 (Hacl.Spec.SHA2.EquivScalar.update_lemma SHA2_256);
-             Lib.Sequence.Lemmas.repeat_blocks_multi_extensionality (block_length SHA2_256)
-               blocks1_raw
-               (Hacl.Spec.SHA2.update SHA2_256)
-               (Lib.UpdateMulti.Lemmas.repeat_f (block_length SHA2_256) (Spec.Agile.Hash.update SHA2_256))
-               st0 }
-        Lib.Sequence.repeat_blocks_multi (block_length SHA2_256) blocks1_raw
-          (Lib.UpdateMulti.Lemmas.repeat_f (block_length SHA2_256) (Spec.Agile.Hash.update SHA2_256))
-          st0;
-      (==) {
-        Lib.UpdateMulti.Lemmas.update_multi_is_repeat_blocks_multi (block_length SHA2_256) (Spec.Agile.Hash.update SHA2_256) st0 blocks1_raw }
-        Lib.UpdateMulti.mk_update_multi (block_length SHA2_256) (Spec.Agile.Hash.update SHA2_256) st0 blocks1_raw;
-      (==) { }
-        Spec.Hash.Incremental.update_last SHA2_256 st0 (prev_len_v prev_len) input0_raw;
-    }
-  end
-
-let update_last_384 st prev_len input input_len =
-  let h0 = ST.get () in
-  [@inline_let]
-  let st' = coerce_to_mb_state SHA2_384 st in
-  [@inline_let]
-  let input' = ntup1 #(Lib.Buffer.lbuffer Lib.IntTypes.uint8 input_len) #1 input in
-  Lib.IntVector.reveal_vec_1 (word_t SHA2_384);
-  [@inline_let]
-  let totlen = prev_len `Hacl.Hash.MD.len_add32 SHA2_384` input_len in
-  Hacl.SHA2.Scalar32.sha384_update_last totlen input_len input' st';
-  let h1 = ST.get () in
-  begin (* ghost *)
-    let input0_raw = B.as_seq h0 input in
-    let input0 = as_seq_multi h0 input' in
-
-    let st0 = as_seq h0 st in
-    let st0' = as_seq #(| SHA2_384, () |) h0 st' in
-    let vlen = Lib.IntTypes.v input_len in
-    let vprev_len = prev_len_v prev_len in
-    let vtotlen = Lib.IntTypes.v totlen in
-    let pad_s = Spec.Hash.MD.pad SHA2_384 vtotlen in
-    let blocks1 = Seq.append input0 pad_s in
-    let blocks1_raw = Seq.append input0_raw pad_s in
-    assert (Seq.length blocks1 % block_length SHA2_384 == 0);
-    assert (Seq.length blocks1_raw % block_length SHA2_384 == 0);
-
-    calc (==) {
-        as_seq h1 st;
-      (==) { }
-        Vec.update_last #SHA2_384 #Vec.M32 totlen vlen input0 st0';
-      (==) { state_spec_v_lemma SHA2_384 (Vec.update_last totlen vlen input0 st0') }
-        Lib.Sequence.index (Vec.state_spec_v #SHA2_384 #Vec.M32 (Vec.update_last totlen vlen input0 st0')) 0;
-      (==) { Hacl.Spec.SHA2.Equiv.update_last_lemma_l #SHA2_384 #Vec.M32 totlen vlen input0 st0' 0 }
-        Hacl.Spec.SHA2.update_last SHA2_384 totlen vlen input0.(|0|)
-          (Lib.Sequence.index (Vec.state_spec_v #SHA2_384 #Vec.M32 st0') 0);
-      (==) { state_spec_v_lemma SHA2_384 st0' }
-        Hacl.Spec.SHA2.update_last SHA2_384 totlen vlen input0.(|0|) st0';
-      (==) { ntup1_lemma #_ #1 input0 }
-        Hacl.Spec.SHA2.update_last SHA2_384 totlen vlen input0 st0';
-      (==) {
-        Hacl.Spec.SHA2.EquivScalar.update_last_is_repeat_blocks_multi SHA2_384 vtotlen vlen input0 st0'
-      }
-        Lib.Sequence.repeat_blocks_multi (block_length SHA2_384) blocks1 (Hacl.Spec.SHA2.update SHA2_384) st0';
-      (==) { assert (st0 `Seq.equal` st0');
-             ntup1_lemma #_ #1 input0; assert (blocks1 `Seq.equal` blocks1_raw) }
-        Lib.Sequence.repeat_blocks_multi (block_length SHA2_384) blocks1_raw (Hacl.Spec.SHA2.update SHA2_384) st0;
-      (==) { Classical.forall_intro_2 (Hacl.Spec.SHA2.EquivScalar.update_lemma SHA2_384);
-             Lib.Sequence.Lemmas.repeat_blocks_multi_extensionality (block_length SHA2_384)
-               blocks1_raw
-               (Hacl.Spec.SHA2.update SHA2_384)
-               (Lib.UpdateMulti.Lemmas.repeat_f (block_length SHA2_384) (Spec.Agile.Hash.update SHA2_384))
-               st0 }
-        Lib.Sequence.repeat_blocks_multi (block_length SHA2_384) blocks1_raw
-          (Lib.UpdateMulti.Lemmas.repeat_f (block_length SHA2_384) (Spec.Agile.Hash.update SHA2_384))
-          st0;
-      (==) {
-        Lib.UpdateMulti.Lemmas.update_multi_is_repeat_blocks_multi (block_length SHA2_384) (Spec.Agile.Hash.update SHA2_384) st0 blocks1_raw }
-        Lib.UpdateMulti.mk_update_multi (block_length SHA2_384) (Spec.Agile.Hash.update SHA2_384) st0 blocks1_raw;
-      (==) { }
-        Spec.Hash.Incremental.update_last SHA2_384 st0 (prev_len_v prev_len) input0_raw;
-    }
-  end
-
-let update_last_512  st prev_len input input_len =
-  let h0 = ST.get () in
-  [@inline_let]
-  let st' = coerce_to_mb_state SHA2_512 st in
-  [@inline_let]
-  let input' = ntup1 #(Lib.Buffer.lbuffer Lib.IntTypes.uint8 input_len) #1 input in
-  Lib.IntVector.reveal_vec_1 (word_t SHA2_512);
-  [@inline_let]
-  let totlen = prev_len `Hacl.Hash.MD.len_add32 SHA2_512` input_len in
-  Hacl.SHA2.Scalar32.sha512_update_last totlen input_len input' st';
-  let h1 = ST.get () in
-  begin (* ghost *)
-    let input0_raw = B.as_seq h0 input in
-    let input0 = as_seq_multi h0 input' in
-
-    let st0 = as_seq h0 st in
-    let st0' = as_seq #(| SHA2_512, () |) h0 st' in
-    let vlen = Lib.IntTypes.v input_len in
-    let vprev_len = prev_len_v prev_len in
-    let vtotlen = Lib.IntTypes.v totlen in
-    let pad_s = Spec.Hash.MD.pad SHA2_512 vtotlen in
-    let blocks1 = Seq.append input0 pad_s in
-    let blocks1_raw = Seq.append input0_raw pad_s in
-    assert (Seq.length blocks1 % block_length SHA2_512 == 0);
-    assert (Seq.length blocks1_raw % block_length SHA2_512 == 0);
-
-    calc (==) {
-        as_seq h1 st;
-      (==) { }
-        Vec.update_last #SHA2_512 #Vec.M32 totlen vlen input0 st0';
-      (==) { state_spec_v_lemma SHA2_512 (Vec.update_last totlen vlen input0 st0') }
-        Lib.Sequence.index (Vec.state_spec_v #SHA2_512 #Vec.M32 (Vec.update_last totlen vlen input0 st0')) 0;
-      (==) { Hacl.Spec.SHA2.Equiv.update_last_lemma_l #SHA2_512 #Vec.M32 totlen vlen input0 st0' 0 }
-        Hacl.Spec.SHA2.update_last SHA2_512 totlen vlen input0.(|0|)
-          (Lib.Sequence.index (Vec.state_spec_v #SHA2_512 #Vec.M32 st0') 0);
-      (==) { state_spec_v_lemma SHA2_512 st0' }
-        Hacl.Spec.SHA2.update_last SHA2_512 totlen vlen input0.(|0|) st0';
-      (==) { ntup1_lemma #_ #1 input0 }
-        Hacl.Spec.SHA2.update_last SHA2_512 totlen vlen input0 st0';
-      (==) {
-        Hacl.Spec.SHA2.EquivScalar.update_last_is_repeat_blocks_multi SHA2_512 vtotlen vlen input0 st0'
-      }
-        Lib.Sequence.repeat_blocks_multi (block_length SHA2_512) blocks1 (Hacl.Spec.SHA2.update SHA2_512) st0';
-      (==) { assert (st0 `Seq.equal` st0');
-             ntup1_lemma #_ #1 input0; assert (blocks1 `Seq.equal` blocks1_raw) }
-        Lib.Sequence.repeat_blocks_multi (block_length SHA2_512) blocks1_raw (Hacl.Spec.SHA2.update SHA2_512) st0;
-      (==) { Classical.forall_intro_2 (Hacl.Spec.SHA2.EquivScalar.update_lemma SHA2_512);
-             Lib.Sequence.Lemmas.repeat_blocks_multi_extensionality (block_length SHA2_512)
-               blocks1_raw
-               (Hacl.Spec.SHA2.update SHA2_512)
-               (Lib.UpdateMulti.Lemmas.repeat_f (block_length SHA2_512) (Spec.Agile.Hash.update SHA2_512))
-               st0 }
-        Lib.Sequence.repeat_blocks_multi (block_length SHA2_512) blocks1_raw
-          (Lib.UpdateMulti.Lemmas.repeat_f (block_length SHA2_512) (Spec.Agile.Hash.update SHA2_512))
-          st0;
-      (==) {
-        Lib.UpdateMulti.Lemmas.update_multi_is_repeat_blocks_multi (block_length SHA2_512) (Spec.Agile.Hash.update SHA2_512) st0 blocks1_raw }
-        Lib.UpdateMulti.mk_update_multi (block_length SHA2_512) (Spec.Agile.Hash.update SHA2_512) st0 blocks1_raw;
-      (==) { }
-        Spec.Hash.Incremental.update_last SHA2_512 st0 (prev_len_v prev_len) input0_raw;
-    }
-  end
+let update_last_224 = mk_update_last SHA2_224
+let update_last_256 = mk_update_last SHA2_256
+let update_last_384 = mk_update_last SHA2_384
+let update_last_512 = mk_update_last SHA2_512
 
 inline_for_extraction noextract
 val mk_finish: a:sha2_alg -> finish_st (| a, () |)
